infoflow: dynamic domain scheduler
No change in the overall property, but the addition of invocations that
can change the domain schedule has the following high-level consequences
for the infoflow proof and infoflow refinement:

- We now explicitly appeal to the (already assumed) absence of domain
  caps to prove that nothing related to the domain schedule can change.
  Previously we could trivially prove this property via crunch over
  the entire kernel without preconditions.

- We add the absence of domain caps to the ADT_if invariants so that
  kernel_entry_if can be shown to preserve domain properties.

Signed-off-by: Gerwin Klein <gerwin.klein@proofcraft.systems>

proof/infoflow/ADT_IF.thy
@@ -792,7 +792,7 @@ lemma kernel_entry_if_invs:
            simp: arch_tcb_update_aux2 ran_tcb_cap_cases)+
 
 lemma kernel_entry_if_globals_equiv:
-  "\<lbrace>invs and (\<lambda>s. e \<noteq> Interrupt \<longrightarrow> ct_active s) and globals_equiv st
+  "\<lbrace>invs and (\<lambda>s. e \<noteq> Interrupt \<longrightarrow> ct_active s) and globals_equiv st and domain_sep_inv irqs st'
          and (\<lambda>s. ct_idle s \<longrightarrow> tc = idle_context s)\<rbrace>
    kernel_entry_if e tc
    \<lbrace>\<lambda>_. globals_equiv st\<rbrace>"
@@ -800,7 +800,7 @@ lemma kernel_entry_if_globals_equiv:
   apply (wp hoare_weak_lift_imp handle_event_globals_equiv
             thread_set_invs_trivial thread_set_context_globals_equiv
          | simp add: ran_tcb_cap_cases arch_tcb_update_aux2)+
-  apply (clarsimp simp: cur_thread_idle)
+  apply (fastforce simp: cur_thread_idle)
   done
 
 lemma thread_set_tcb_context_update_neg_cte_wp_at[wp]:
@@ -819,10 +819,6 @@ lemma thread_set_tcb_context_update_neg_cte_wp_at[wp]:
    apply (fastforce simp: tcb_cap_cases_def split: if_splits)
   apply (fastforce elim: cte_wp_atE intro: cte_wp_at_cteI cte_wp_at_tcbI)
   done
-
-lemma thread_set_tcb_context_update_domain_sep_inv[wp]:
-  "thread_set (tcb_arch_update f) t \<lbrace>domain_sep_inv irqs st\<rbrace>"
-  by (wp domain_sep_inv_triv)
 
 
 subsection \<open>handle_preemption_if\<close>
@@ -954,7 +950,7 @@ locale ADT_IF_1 =
     "(Some irq, s') \<in> fst (do_machine_op (getActiveIRQ in_kernel) s)
      \<Longrightarrow> irq_at (irq_state (machine_state s) + 1) (irq_masks (machine_state s)) = Some irq"
   and kernel_entry_if_idle_equiv:
-    "\<lbrace>invs and (\<lambda>s. e \<noteq> Interrupt \<longrightarrow> ct_active s) and idle_equiv st
+    "\<lbrace>invs and (\<lambda>s. e \<noteq> Interrupt \<longrightarrow> ct_active s) and domain_sep_inv irqs st and idle_equiv st
            and (\<lambda>s. ct_idle s \<longrightarrow> tc = idle_context s)\<rbrace>
      kernel_entry_if e tc
      \<lbrace>\<lambda>_. idle_equiv st\<rbrace>"
@@ -1007,6 +1003,9 @@ locale ADT_IF_1 =
        \<Longrightarrow> thread_set f t \<lbrace>pas_refined aag\<rbrace>"
 begin
 
+lemmas do_user_op_if_no_domain_caps[wp] =
+  no_domain_caps_sep_inv_lift[OF do_user_op_if_domain_sep_inv]
+
 lemma kernel_entry_silc_inv[wp]:
   "\<lbrace>silc_inv aag st and einvs and simple_sched_action and (\<lambda>s. ev \<noteq> Interrupt \<longrightarrow> ct_active s)
                     and pas_refined (aag :: 'a subject_label PAS)
@@ -1040,6 +1039,9 @@ lemma kernel_entry_if_domain_sep_inv:
                wp: handle_event_domain_sep_inv hoare_weak_lift_imp
                    thread_set_invs_trivial thread_set_not_state_valid_sched)+
 
+lemmas kernel_entry_if_no_domain_caps[wp] =
+  no_domain_caps_sep_inv_lift_r2[OF kernel_entry_if_domain_sep_inv]
+
 lemma kernel_entry_if_valid_sched:
   "\<lbrace>valid_sched and invs and (ct_active or ct_idle)
                 and (\<lambda>s. (e \<noteq> Interrupt \<longrightarrow> ct_active s) \<and> scheduler_action s = resume_cur_thread)\<rbrace>
@@ -1056,6 +1058,11 @@ lemma kernel_entry_if_irq_masks:
    \<lbrace>\<lambda>_ s. P (irq_masks_of_state s)\<rbrace>"
   by (simp add: kernel_entry_if_def ran_tcb_cap_cases arch_tcb_update_aux2
       | wp handle_event_irq_masks thread_set_invs_trivial | force)+
+
+lemma kernel_entry_if_valid_domain_list[wp]:
+  "\<lbrace>valid_domain_list and invs\<rbrace> kernel_entry_if e tc \<lbrace>\<lambda>_. valid_domain_list\<rbrace>"
+  unfolding kernel_entry_if_def
+  by (wpsimp wp: thread_set_invs_trivial simp: ran_tcb_cap_cases arch_tcb_update_aux2)
 
 crunch schedule_if
   for pas_refined[wp]: "pas_refined aag"
@@ -1111,6 +1118,9 @@ lemma handle_preemption_if_domain_sep_inv:
     apply (wpsimp wp: getActiveIRQ_rv_None)+
   done
 
+lemmas handle_preemption_if_no_domain_caps[wp] =
+  no_domain_caps_sep_inv_lift[OF handle_preemption_if_domain_sep_inv]
+
 lemma handle_kernel_interrupt_pas_refined:
   "\<lbrace>pas_refined aag and K (irq \<notin> non_kernel_IRQs)\<rbrace>
    handle_interrupt irq
@@ -1130,6 +1140,11 @@ lemma handle_preemption_if_pas_refined[wp]:
                 in hoare_strengthen_post)
     apply (wpsimp wp: getActiveIRQ_rv_None)+
   done
+
+lemma handle_preemption_if_valid_domain_list[wp]:
+  "handle_preemption_if tc \<lbrace>valid_domain_list\<rbrace>"
+  unfolding handle_preemption_if_def
+  by (wpsimp wp: valid_domain_list_lift)
 
 end
 
@@ -1364,7 +1379,7 @@ abbreviation internal_state_if :: "'a global_sys_state \<Rightarrow> 'a" where
 (*Weakened invs_if to properties only necessary for refinement*)
 definition full_invs_if :: "observable_if set" where
   "full_invs_if \<equiv>
-     {s. einvs (internal_state_if s) \<and>
+     {s. einvs (internal_state_if s) \<and> no_domain_caps (internal_state_if s) \<and>
          (snd s \<noteq> KernelSchedule True \<longrightarrow> domain_time (internal_state_if s) > 0) \<and>
          (domain_time (internal_state_if s) = 0
           \<longrightarrow> scheduler_action (internal_state_if s) = choose_new_thread) \<and>
@@ -1571,8 +1586,6 @@ crunch handle_yield
   for domain_fields[wp]: "domain_fields P"
 crunch activate_thread
   for domain_fields[wp]: "domain_fields P"
-crunch kernel_entry_if
-  for domain_list[wp]: "\<lambda>s::det_state. P (domain_list s)"
 crunch handle_preemption_if
   for domain_list[wp]: "\<lambda>s::det_state. P (domain_list s)"
 crunch schedule_if
@@ -1604,39 +1617,84 @@ lemma schedule_if_domain_time_nonzero:
   apply simp
   done
 
+lemma schedule_if_valid_domain_list[wp]:
+  "schedule_if tc \<lbrace>valid_domain_list\<rbrace>"
+  unfolding schedule_if_def
+  by (wpsimp wp: valid_domain_list_lift)
+
+lemma invoke_domain_false:
+  "\<lbrace>\<bottom>\<rbrace> invoke_domain di \<lbrace>Q\<rbrace>"
+  by wpsimp
+
+lemma perform_invocation_domain_time_inv:
+  "\<lbrace>(\<lambda>s. P (domain_time s)) and no_domain_caps and K (no_domain_inv iv)\<rbrace>
+   perform_invocation block call iv
+   \<lbrace>\<lambda>_ s::det_state. P (domain_time s)\<rbrace>"
+  unfolding no_domain_inv_def
+  by (cases iv; wpsimp wp: invoke_domain_false)
+
+lemma perform_invocation_domain_time_sep_inv:
+  "\<lbrace>(\<lambda>s. P (domain_time s)) and domain_sep_inv irqs st' and authorised_for_globals_inv iv\<rbrace>
+   perform_invocation block call iv
+   \<lbrace>\<lambda>_ s::det_state. P (domain_time s)\<rbrace>"
+  unfolding authorised_for_globals_inv_def
+  apply (wp perform_invocation_domain_time_inv)
+  apply (cases iv; clarsimp simp: no_domain_caps_strg)
+  done
+
+lemma handle_invocation_domain_time_inv:
+  "\<lbrace>(\<lambda>s. P (domain_time s)) and invs and no_domain_caps\<rbrace>
+   handle_invocation calling blocking
+   \<lbrace>\<lambda>_ s::det_state. P (domain_time s)\<rbrace>"
+  unfolding handle_invocation_def
+  by (wpsimp wp: perform_invocation_domain_time_inv
+                 no_domain_caps_sep_inv_lift[OF set_thread_state_domain_sep_inv]
+                 decode_invocation_no_domain_inv
+                 syscall_valid hoare_drop_imps
+             simp: prod_imp_fst_snd o_def
+             simp_del: split_paired_All)
+
+lemma maybe_handle_interrupt_false:
+  "\<lbrace>\<bottom>\<rbrace> maybe_handle_interrupt in_kernel \<lbrace>Q\<rbrace>"
+  by wpsimp
+
+lemma handle_event_noIRQ_domain_time_inv:
+  "e \<noteq> Interrupt \<Longrightarrow>
+   \<lbrace>invs and no_domain_caps and (\<lambda>s. P (domain_time s)) \<rbrace>
+   handle_event e
+   \<lbrace>\<lambda>_ s::det_state. P (domain_time s)\<rbrace>"
+  by (cases e; wpsimp wp: maybe_handle_interrupt_false handle_invocation_domain_time_inv
+                      simp: handle_call_def handle_send_def)
+
+lemma kernel_entry_if_noIRQ_domain_time_inv:
+  "e \<noteq> Interrupt \<Longrightarrow>
+   \<lbrace>invs and no_domain_caps and (\<lambda>s. P (domain_time s))\<rbrace>
+   kernel_entry_if e tc
+   \<lbrace>\<lambda>_ s. P (domain_time s)\<rbrace>"
+  unfolding kernel_entry_if_def
+  by (wpsimp wp: handle_event_noIRQ_domain_time_inv thread_set_invs_trivial
+                 no_domain_caps_sep_inv_lift
+             simp: ran_tcb_cap_cases arch_tcb_update_aux2)
+
+lemma kernel_entry_if_noIRQ_domain_time_sep_inv:
+  "e \<noteq> Interrupt \<Longrightarrow>
+   \<lbrace>invs and domain_sep_inv irqs st and (\<lambda>s. P (domain_time s))\<rbrace>
+   kernel_entry_if e tc
+   \<lbrace>\<lambda>_ s. P (domain_time s)\<rbrace>"
+  by (wpsimp wp: kernel_entry_if_noIRQ_domain_time_inv simp: no_domain_caps_strg)
 
 context ADT_IF_1 begin
-
-lemma handle_event_domain_fields:
-  "\<lbrace>domain_fields P and K (e \<noteq> Interrupt)\<rbrace>
-   handle_event e
-   \<lbrace>\<lambda>_. domain_fields P\<rbrace>"
-  apply (rule hoare_gen_asm)
-  apply (rule hoare_pre)
-   apply (case_tac e)
-        apply (rename_tac syscall)
-        apply (case_tac syscall)
-               apply (wp | simp add: handle_call_def)+
-  done
-
-lemma kernel_entry_if_domain_fields:
-  "\<lbrace>domain_fields P and K (e \<noteq> Interrupt)\<rbrace>
-   kernel_entry_if e tc
-   \<lbrace>\<lambda>_. domain_fields P\<rbrace>"
-  apply (simp add: kernel_entry_if_def)
-  apply (wp handle_event_domain_fields | simp)+
-  done
 
 lemma kernel_entry_if_domain_time_sched_action:
   "\<lbrace>\<lambda>s. domain_time s > 0\<rbrace>
    kernel_entry_if e tc
    \<lbrace>\<lambda>_ s. domain_time s = 0 \<longrightarrow> scheduler_action s = choose_new_thread\<rbrace>"
+  unfolding kernel_entry_if_def
   apply (case_tac "e = Interrupt")
    apply (simp add: kernel_entry_if_def maybe_handle_interrupt_def)
    apply (wp handle_interrupt_valid_domain_time| wpc | simp)+
       apply (rule_tac Q'="\<lambda>r s. domain_time s > 0" in hoare_strengthen_post)
-       apply (wp | simp)+
-      apply (wp hoare_false_imp kernel_entry_if_domain_fields | fastforce)+
+       apply wpsimp+
   done
 
 end
@@ -2000,8 +2058,9 @@ lemma invs_if_Step_ADT_A_if:
                        kernel_entry_pas_refined[where st=s0_internal]
                        kernel_entry_if_valid_sched kernel_entry_if_only_timer_irq_inv
                        kernel_entry_if_domain_sep_inv kernel_entry_if_guarded_pas_domain
-                       kernel_entry_if_domain_fields kernel_entry_if_idle_equiv
+                       kernel_entry_if_idle_equiv
                        kernel_entry_if_domain_time_sched_action
+                       kernel_entry_if_noIRQ_domain_time_sep_inv
                        hoare_false_imp ct_idle_lift
                     | clarsimp intro!: guarded_pas_is_subject_current_aag[rule_format]
                     | intro conjI)+
@@ -2031,12 +2090,14 @@ lemma invs_if_Step_ADT_A_if:
                       kernel_entry_if_valid_sched kernel_entry_if_only_timer_irq_inv
                       kernel_entry_if_domain_sep_inv kernel_entry_if_guarded_pas_domain
                       kernel_entry_if_domain_time_sched_action
+                      kernel_entry_if_noIRQ_domain_time_sep_inv
                       ct_idle_lift
-                   | clarsimp intro: guarded_pas_is_subject_current_aag
-                   | wp kernel_entry_if_domain_fields)+
+                   | clarsimp intro: guarded_pas_is_subject_current_aag)+
           apply (rule conjI, fastforce intro!: active_from_running)
           apply (simp add: schact_is_rct_def)
-          apply (rule guarded_pas_is_subject_current_aag,assumption+)
+          apply (rule conjI)
+           apply (rule guarded_pas_is_subject_current_aag,assumption+)
+          apply fastforce
          apply (simp_all only: silc_inv_cur pas_refined_cur guarded_pas_domain_cur)
          apply (simp | elim exE)+
          apply (elim exE conjE)
@@ -2178,7 +2239,7 @@ context valid_initial_state begin
 
 lemma invs_if_full_invs_if:
   "invs_if s \<Longrightarrow> s \<in> full_invs_if"
-  by (clarsimp simp: full_invs_if_def invs_if_def Invs_def)
+  by (clarsimp simp: full_invs_if_def invs_if_def Invs_def no_domain_caps_strg)
 
 end
 
@@ -2594,11 +2655,10 @@ lemma checked_insert_irq_state_of_state[wp]:
   by (wp | simp add: check_cap_at_def)+
 
 lemma irq_state_inv_invoke_domain[wp]:
-  "invoke_domain a b \<lbrace>irq_state_inv st\<rbrace>"
+  "invoke_domain di \<lbrace>irq_state_inv st\<rbrace>"
   apply (simp add: irq_state_inv_def[abs_def])
-  apply (rule hoare_pre)
-   apply wps
-   apply (wp | clarsimp)+
+  apply (wp_pre, wps, wpsimp)
+  apply clarsimp
   done
 
 crunch bind_notification
