proof/infoflow/RISCV64/Example_Valid_State.thy
@@ -826,6 +826,7 @@ definition s0_internal :: "det_ext state" where
      scheduler_action = resume_cur_thread,
      domain_list = [(0, 10), (1, 10)],
      domain_index = 0,
+     domain_start_index = 0,
      cur_domain = 0,
      domain_time = 5,
      ready_queues = (const (const [])),
